define some ghost_proof assertions and verify their properties

src/program_proof/pb/ghost_proof.v
@@ -4,13 +4,15 @@ From Perennial.program_proof Require Import grove_prelude.
 (*
   "Gauge-invariant" part of the proof
  *)
-Local Definition cn_logR := gmapR u64 (mono_listR (leibnizO u64)).
-Local Definition cn_rep_logR := gmapR u64 (mono_listR (leibnizO u64)).
+Local Definition logR := mono_listR (leibnizO u8).
+Local Definition cn_logR := gmapR u64 logR.
+Local Definition cn_rep_logR := gmapR (u64*u64) logR.
 Class pb_ghostG Σ :=
-  { pb_ghost_cn_logG :> inG Σ cn_logR;
+  { pb_ghost_logG :> inG Σ logR;
+    pb_ghost_cn_logG :> inG Σ cn_logR;
     pb_ghost_cn_rep_logG :> inG Σ cn_rep_logR }.
 
-Definition pb_ghostΣ := #[GFunctor cn_logR; GFunctor cn_rep_logR].
+Definition pb_ghostΣ := #[GFunctor logR; GFunctor cn_logR; GFunctor cn_rep_logR].
 
 Global Instance subG_pb_ghostG {Σ} :
   subG pb_ghostΣ Σ → pb_ghostG Σ.
@@ -18,7 +20,9 @@ Proof. solve_inG. Qed.
 
 Record pb_names :=
   {
-  commit_gn:gname
+  pb_proposal_gn : gname;
+  pb_accepted_gn : gname;
+  pb_commit_gn : gname;
   }.
 
 Definition Log := list u8.
@@ -38,30 +42,30 @@ Implicit Type γ : pb_names.
 Definition config_ptsto γ (cn:u64) (conf:list u64): iProp Σ.
 Admitted.
 
-Definition proposal_ptsto γ (cn:u64) (l:Log): iProp Σ.
-Admitted.
-
-Definition proposal_lb γ (cn:u64) (l:Log): iProp Σ.
-Admitted.
+Definition proposal_ptsto γ (cn:u64) (l:Log): iProp Σ :=
+  own γ.(pb_proposal_gn) {[cn := ●ML (l : list (leibnizO u8))]}.
 
 (* Probably not needed *)
-Definition proposal_ptsto_ro γ (cn:u64) (l:Log): iProp Σ.
-Admitted.
+(* Definition proposal_ptsto_ro γ (cn:u64) (l:Log): iProp Σ.
+Admitted. *)
 
-Definition accepted_ptsto γ (cn:u64) (r:u64) (l:Log): iProp Σ.
-Admitted.
+Definition proposal_lb γ (cn:u64) (l:Log): iProp Σ :=
+  own γ.(pb_proposal_gn) {[cn := ◯ML (l : list (leibnizO u8))]}.
 
-Definition accepted_lb γ (cn:u64) (r:u64) (l:Log): iProp Σ.
-Admitted.
+Definition accepted_ptsto γ (cn:u64) (r:u64) (l:Log): iProp Σ :=
+  own γ.(pb_accepted_gn) {[(cn,r) := ●ML (l : list (leibnizO u8))]}.
 
-Definition accepted_ptsto_ro γ (cn:u64) (r:u64) (l:Log): iProp Σ.
-Admitted.
+Definition accepted_ptsto_ro γ (cn:u64) (r:u64) (l:Log): iProp Σ :=
+  own γ.(pb_accepted_gn) {[(cn,r) := ●□ML (l : list (leibnizO u8))]}.
 
-Definition commit_ptsto γ (l:Log): iProp Σ.
-Admitted.
+Definition accepted_lb γ (cn:u64) (r:u64) (l:Log): iProp Σ :=
+  own γ.(pb_accepted_gn) {[(cn,r) := ◯ML (l : list (leibnizO u8))]}.
 
-Definition commit_lb γ (l:Log): iProp Σ.
-Admitted.
+Definition commit_ptsto γ (l:Log): iProp Σ :=
+  own γ.(pb_commit_gn) (●ML (l : list (leibnizO u8))).
+
+Definition commit_lb γ (l:Log): iProp Σ :=
+  own γ.(pb_commit_gn) (◯ML (l : list (leibnizO u8))).
 
 Global Instance config_ptsto_pers γ cn conf :
   Persistent (config_ptsto γ cn conf).
@@ -69,15 +73,15 @@ Admitted.
 
 Global Instance proposal_lb_pers γ cn l :
   Persistent (proposal_lb γ cn l).
-Admitted.
+Proof. apply _. Qed.
 
 Global Instance accepted_lb_pers γ cn r l :
   Persistent (accepted_lb γ cn r l).
-Admitted.
+Proof. apply _. Qed.
 
 Global Instance committed_lb_pers γ l :
   Persistent (commit_lb γ l).
-Admitted.
+Proof. apply _. Qed.
 
 Definition accepted_by γ cn l : iProp Σ :=
   ∃ conf, config_ptsto γ cn conf ∗
@@ -87,6 +91,9 @@ Definition oldConfMax γ (cn:u64) log : iProp Σ :=
   □(∀ cn_old log_old ,
    ⌜int.Z cn_old < int.Z cn⌝ →
    accepted_by γ cn_old log_old → ⌜log_old ⪯ log⌝).
+
+Definition commit_lb_by γ (cn:u64) l : iProp Σ :=
+  commit_lb γ l ∗ (∃ cn_old, ⌜int.Z cn_old <= int.Z cn⌝ ∗ accepted_by γ cn_old l).
 
 (* Want better name *)
 Definition proposal_lb_fancy γ cn log : iProp Σ :=
@@ -109,25 +116,41 @@ Admitted.
 Lemma accepted_update γ cn r l l' :
   (l ⪯ l') → accepted_ptsto γ cn r l ==∗ accepted_ptsto γ cn r l'.
 Proof.
-Admitted.
+  iIntros (Hll'). iApply own_update.
+  apply singleton_update, mono_list_update.
+  done.
+Qed.
 
 Lemma accepted_witness γ cn r l :
   accepted_ptsto γ cn r l -∗ accepted_lb γ cn r l.
 Proof.
-Admitted.
+  iApply own_mono.
+  apply singleton_mono, mono_list_included.
+Qed.
 
 Lemma accepted_lb_monotonic γ cn r l l':
   l ⪯ l' → accepted_lb γ cn r l' -∗ accepted_lb γ cn r l.
 Proof.
-Admitted.
+  iIntros (Hll'). iApply own_mono.
+  apply singleton_mono, mono_list_lb_mono.
+  done.
+Qed.
 
 Lemma proposal_lb_comparable γ cn l l' :
+  proposal_lb γ cn l -∗ proposal_lb γ cn l' -∗ ⌜l ⪯ l' ∨  l' ⪯ l⌝.
+Proof.
+  iIntros "Hl Hl'".
+  iDestruct (own_valid_2 with "Hl Hl'") as %Hval.
+  iPureIntro. revert Hval.
+  rewrite singleton_op singleton_valid => /mono_list_lb_op_valid_L.
+  done.
+Qed.
+
+Lemma proposal_lb_fancy_comparable γ cn l l' :
   proposal_lb_fancy γ cn l -∗ proposal_lb_fancy γ cn l' -∗ ⌜l ⪯ l' ∨  l' ⪯ l⌝.
 Proof.
-Admitted.
-
-Definition commit_lb_by γ (cn:u64) l : iProp Σ :=
-  commit_lb γ l ∗ (∃ cn_old, ⌜int.Z cn_old <= int.Z cn⌝ ∗ accepted_by γ cn_old l).
+  iIntros "[Hl _] [Hl' _]". iApply (proposal_lb_comparable with "Hl Hl'").
+Qed.
 
 (* commit_lb_by is covariant in cn, contravariant in l *)
 Lemma commit_lb_by_monotonic γ cn cn' l l' :
@@ -152,3 +175,5 @@ Proof.
 Admitted.
 
 End definitions.
+
+Typeclasses Opaque proposal_ptsto proposal_lb accepted_ptsto accepted_ptsto_ro accepted_lb commit_ptsto commit_lb.
